src/FP/Classes/Monad.v
@@ -1,27 +1,19 @@
 Require Import FP.Data.WeakSetoid.
 Require Import FP.Classes.WeakEqv.
+Require Import FP.Classes.Applicative.
+Require Import FP.Classes.Eqv.
 Require Import FP.Data.Function_Q.
+Require Import FP.Data.Relation.
 Require Import FP.Data.Unit.
 Require Import FP.Data.Function.
+Require Import FP.Data.RewriteState.
 
 Import Eqv.Notation.
 Import WeakSetoid.Notation.
 Import Unit.Notation.
 Import Function.Notation.
 Import WeakEqv.Notation.
-
-Definition bind_associativity_k 
-  {m:WeakSetoid -> WeakSetoid} (bind:forall {A B:WeakSetoid}, DD (m A ⇨ (A ⇨ m B) ⇨ m B)) 
-  {A B C:WeakSetoid} (f:DD (A ⇨ m B)) (g:DD (B ⇨ m C))
-  : DD (A ⇨ m C) := 
-    mk_DD_infer (A ⇨ m C) 
-                (fun x => DD_value bind (DD_value f x) (DD_value g)).
-
-(* consider changing A ⇨ B to have DD A -> DD B as underlying type,
-   rather than A -> B.  This is so arbitrary contexts (like the one
-   created above, fun x => DD_value bind ...)  can give good beta
-   rules.  After thinking about it, this sounds like the right way to
-   go, and doesn't contradict anything I've built so far. *)
+Import RewriteState.Notation.
 
 Class Monad (m:WeakSetoid -> WeakSetoid) : Type :=
   { ret : 
@@ -38,8 +30,48 @@ Class Monad (m:WeakSetoid -> WeakSetoid) : Type :=
   ; monad_associativity :
       forall {A B C:WeakSetoid} (xM:DD (m A)) (f:DD (A ⇨ m B)) (g:DD (B ⇨ m C)),
       bind ⊛ (bind ⊛ xM ⊛ f) ⊛ g 
-      ≃ bind ⊛ xM ⊛ bind_associativity_k (@bind) f g
+      ≃ bind ⊛ xM ⊛ (λ x → bind ⊛ (f ⊛ x) ⊛ g)
   }.
+Ltac R_Monad_left_unit :=
+  match goal with
+  | [ |- RewriteState (bind ⊛ ?xM ⊛ ret) _ _ ] => ReplaceBy (monad_left_unit xM)
+  end.
+Ltac R_Monad_right_unit :=
+  match goal with
+  | [ |- RewriteState (bind ⊛ (ret ⊛ ?x) ⊛ ?k) _ _ ] => ReplaceBy (monad_right_unit x k)
+  end.
+Ltac R_Monad_associativity :=
+  match goal with
+  | [ |- RewriteState (bind ⊛ (bind ⊛ ?xM ⊛ ?f) ⊛ ?g) _ _ ] => ReplaceBy (monad_associativity xM f g)
+  end.
+Ltac R_Monad := R_Monad_left_unit || R_Monad_right_unit || R_Monad_associativity.
+
+Section Monad.
+  Context {m:WeakSetoid -> WeakSetoid} `{! Monad m }.
+  
+  Definition monad_fapply {A B:WeakSetoid} : DD (m (A ⇨ B) ⇨ m A ⇨ m B) :=
+    λ fM → λ xM → bind ⊛ fM ⊛ (λ f → bind ⊛ xM ⊛ (λ x → ret ⊛ (f ⊛ x))).
+  
+  Local Instance Monad_To_Applicative : Applicative m := { fret := @ret _ _ ; fapply := @monad_fapply }.
+  Proof.
+    Local Ltac Hammer := 
+      intros ; unfold monad_fapply,fret,mk_DD_infer_f ;
+      repeat Everywhere ltac:(R_fun_beta || R_Monad).
+    - Hammer.
+
+      
+      unfold_eqv ; unfold_weqv ; unfold respectful ; intros.
+      e1 ≈ e1
+      λ x → e1 ≈ λ x → e2
+      intros ; unfold monad_fapply,fret,mk_DD_infer_f.
+      unfold "≃" ; simpl.
+      decide_weqv.
+      Hammer.
+      Enter.
+      R_beta.
+      PushFun.
+      Hammer.
+End Monad.
 
 Class MonadState (S:WeakSetoid) (m:WeakSetoid -> WeakSetoid) : Type :=
   { get : DD (m S)
@@ -52,5 +84,5 @@ Class MonadPlus (m:WeakSetoid -> WeakSetoid) `{! Monad m } : Type :=
       DD (m A ⇨ m A ⇨ m A) 
   ; monad_plus_distributivity : 
       forall {A B:WeakSetoid} (xM yM:DD (m A)) (k:DD (A ⇨ m B)), 
-      extend ⊛ k ⊛ (mplus ⊛ xM ⊛ yM) ≃ mplus ⊛ (extend ⊛ k ⊛ xM) ⊛ (extend ⊛ k ⊛ yM)
+
   }.
