src/FP/Data/WeakSetoid.v
@@ -1,11 +1,14 @@
 Require Import FP.Classes.WeakEqv.
 Require Import FP.Classes.Eqv.
+Require Import FP.Classes.Symmetric.
+Require Import FP.Classes.Transitive.
 Require Import FP.Data.Relation.
 Require Import FP.Data.Function.
 Require Import FP.Classes.Reflexive.
 Require Import FP.Classes.Symmetric.
 Require Import FP.Classes.Transitive.
 Require Import FP.Data.Type.
+Require Import FP.Data.Tactic.
 
 Import Relation.Notation.
 Import Function.Notation.
@@ -18,6 +21,10 @@ Inductive WeakSetoid : Type := mk_WeakSetoid
   }.
 Existing Instance WeakSetoid_WeakEqv.
 
+(* Embed a type with Leibniz equality *)
+Definition EL (A:Type) : WeakSetoid := mk_WeakSetoid A (Leibniz_WeakEqv A).
+
+(* Domain of definition for a weak setoid. *)
 Inductive DD (A:WeakSetoid) : Type := mk_DD
   { DD_value : WeakSetoid_T A
   ; DD_proper : proper weqv DD_value
@@ -25,8 +32,9 @@ Inductive DD (A:WeakSetoid) : Type := mk_DD
 Arguments DD_value {A} _.
 Arguments DD_proper {A} _.
 
+(* Equivalence relation over values in DD *)
 Instance DD_Eqv {A:WeakSetoid} : Eqv (DD A) :=
-  { eqv x y := (DD_value x ≈ DD_value y) }.
+  { eqv x y := DD_value x ≈ DD_value y }.
 Proof.
   - econstructor ; intros.
     apply (DD_proper x).
@@ -35,59 +43,98 @@ Proof.
   - econstructor ; intros.
     Transitivity (DD_value y) ; auto.
 Defined.
+(* Induced weak equivalence *)
+Instance DD_WeakEqv {A:WeakSetoid} : WeakEqv (DD A) := Eqv_WeakEqv.
 
+(* Arrows in the weak setoid universe *)
 Definition weak_setoid_arrow (A B:WeakSetoid) : WeakSetoid :=
-  mk_WeakSetoid (WeakSetoid_T A -> WeakSetoid_T B) Function_WeakEqv.
+  mk_WeakSetoid (DD A -> DD B) Function_WeakEqv.
 Local Infix "⇨" := weak_setoid_arrow (right associativity, at level 100).
 
+(* Application *)
 Definition weak_setoid_apply {A B:WeakSetoid} (f:DD (A ⇨ B)) (x:DD A) : DD B :=
-  mk_DD B (DD_value f $ DD_value x) (DD_proper f (DD_value x) (DD_value x) (DD_proper x)).
+  mk_DD B (DD_value $ DD_value f $ x) (DD_proper f x x (DD_proper x)).
 Local Infix "⊛" := weak_setoid_apply (left associativity, at level 50).
 
-Definition EL (A:Type) : WeakSetoid := mk_WeakSetoid A (Leibniz_WeakEqv A).
+(* Lambdas *)
+Definition mk_DD_f {A B:WeakSetoid} (f:DD A -> DD B) (p:proper weqv f) : DD (A ⇨ B) :=
+  mk_DD (A ⇨ B) f p.
+Local Notation "'λ?'  x .. y → e" := 
+  (mk_DD_f (fun x => .. (mk_DD_f (fun y => e) _) ..) _)
+  (right associativity, at level 200, x binder, y binder).
 
-Ltac finish_decide_weqv_proper :=
-  match goal with
-  | [ |- ?f ?x ≈ ?g ?y ] => apply function_weqv_app ; finish_decide_weqv_proper
-  | [ |- DD_value ?x ≈ DD_value ?x ] => exact (DD_proper x)
-  | _ => tauto
-  end.
+(* Respect introduction for _⇨_ *)
+Definition weak_setoid_respect_intro {A B:WeakSetoid}
+  {f g:DD (A ⇨ B)} (p:forall x y, x ≃ y -> f ⊛ x ≃ g ⊛ y)
+  : f ≃ g := p.
 
-Ltac decide_weqv_proper :=
-  repeat
-    (try finish_decide_weqv_proper ;
-     match goal with
-     | [ |- proper _ _ ] => unfold proper
-     | [ |- ?f ≈ ?g ] =>
-         match type of f with _ -> _ => 
-           unfold "≈" ; simpl ; unfold respectful ; intros ; simpl
-         end
-     end).
+(* Respect elimination for _⇨_ *)
+Definition weak_setoid_respect_elim {A B:WeakSetoid} 
+  {f g:DD (A ⇨ B)} (pf:f ≃ g) (x y:DD A) (px:x ≃ y)
+  : f ⊛ x ≃ g ⊛ y := pf x y px.
+
+(* Beta rule *)
+Definition weak_setoid_beta {A B:WeakSetoid}
+  (f:DD A -> DD B) (p:proper weqv f) (e:DD A)
+  : mk_DD_f f p ⊛ e ≃ f e := p e e reflexivity.
+
+Section Relation.
+  Context {T} {R:relation T} `{! Symmetric R ,! Transitive R }.
+  Definition replace_left {x y z} : R x y -> R y z -> R x z := transitivity y.
+  Definition replace_right {x y z} : R y z -> R x z -> R x y := fun yRz xRz => transitivity z xRz (symmetry yRz).
+End Relation.
 
 Class ByDecideWeqv {A:WeakSetoid} (x:WeakSetoid_T A) : Type := 
   by_decide_weqv : proper weqv x.
-Hint Extern 5 =>
-  match goal with
-  | [ |- ByDecideWeqv ?x ] => 
-      unfold ByDecideWeqv ; decide_weqv_proper
-  end : typeclass_instances.
-
 Definition mk_DD_infer (A:WeakSetoid) (x:WeakSetoid_T A) `{! ByDecideWeqv x } : DD A :=
   mk_DD A x by_decide_weqv.
+Definition mk_DD_infer_f {A B:WeakSetoid} (f:DD A -> DD B) `{! ByDecideWeqv (A:=A ⇨ B) f } : DD (A ⇨ B) :=
+  mk_DD_f f $ by_decide_weqv (A:=A ⇨ B).
 
-Ltac decide_weqv_beta :=
-  repeat
+Ltac decide_weqv :=
+  repeat (
+    unfold mk_DD_infer_f ;
     match goal with
-    | [ |- ?x ≃ ?y ] =>
-        match type of x with DD _ =>
-          unfold "≃" ; simpl
-        end
-    | [ |- DD_value ?x ≈ DD_value ?x ] => apply (DD_proper x)
-    | [ |- DD_value ?f _ ≈ DD_value ?f _ ] => apply (DD_proper f)
-    end ;
+    | [ |- ByDecideWeqv _ ] => unfold ByDecideWeqv
+    | [ |- proper _ _ ] => unfold proper
+    | [ |- ?x ≈ ?y ] => match type of x with DD _ => change (x ≃ y) end
+    | [ |- (fun _ => _) ≈ (fun _ => _) ] => eapply fun_respect_intro ; intros
+    | [ |- (λ? _ → _) ≃ (λ? _ → _) ] =>
+      (*
+        eapply weak_setoid_respect_intro ; intros ;
+        eapply (replace_left (weak_setoid_beta _ _ _)) ;
+        eapply (replace_right (weak_setoid_beta _ _ _))
+*)
+        eapply weak_setoid_respect_intro ; intros ;
+        match goal with
+        | [ |- ?e1 ≃ ?e2 ] =>
+            let e1' := eval red in e1 in
+            let e2' := eval red in e2 in
+            change (e1' ≃ e2')
+        end ; simpl
+    | [ |- _ ⊛ _ ≃ _ ⊛ _ ] => eapply weak_setoid_respect_elim
+    | [ |- _ ≃ _ ] => Reflexivity
+                                  (*
+    | [ |- (fun x => _) ≈ (fun y => _) ] => unfold_weqv ; unfold respectful ; intros
+    | [ |- {| DD_value := fun x => _ ; DD_proper := _ |} ≈ {| DD_value := fun y => _ ; DD_proper := _ |} ] =>
+        unfold_weqv ; unfold_eqv ; cbv delta [DD_value] beta iota
+    | [ |- ?f ⊛ _ ≈ ?g ⊛ _ ] => apply weak_setoid_apply_respect
+    | [ |- ?f _ ≈ ?g _ ] => apply function_weqv_app
+    | [ x : DD _ |- ?x ≈ ?x ] => apply (DD_proper x)
+    | [ |- mk_DD_infer_f _ ≈ mk_DD_infer_f _ ] => unfold mk_DD_infer_f
+    | [ |- mk_DD_f _ _ ≈ mk_DD_f _ _ ] => unfold mk_DD_f
+*)
+    end) ; 
   auto.
+Hint Extern 9 => (decide_weqv ; tauto) : typeclass_instances.
 
 Module Notation.
   Infix "⇨" := weak_setoid_arrow (right associativity, at level 100).
   Infix "⊛" := weak_setoid_apply (left associativity, at level 50).
+  Notation "'λ'  x .. y → e" := 
+    (mk_DD_infer_f (fun x => .. (mk_DD_infer_f (fun y => e)) ..))
+    (right associativity, at level 200, x binder, y binder).
+  Notation "'λ?'  x .. y → e" := 
+    (mk_DD_f (fun x => .. (mk_DD_f (fun y => e) _) ..) _)
+    (right associativity, at level 200, x binder, y binder).
 End Notation.
