src/FP/Classes/Eqv.v
@@ -1,6 +1,7 @@
 Require Import FP.Classes.Reflexive.
 Require Import FP.Classes.Symmetric.
 Require Import FP.Classes.Transitive.
+Require Import FP.Classes.WeakEqv.
 
 Class Eqv (A:Type) : Type :=
   { eqv : A -> A -> Type
@@ -9,6 +10,21 @@ Class Eqv (A:Type) : Type :=
   ; Eqv_Transitive :> Transitive eqv
   }.
 Arguments eqv {A} {Eqv} _ _ : simpl never.
+
+Ltac unfold_eqv :=
+  unfold eqv ;
+  match goal with
+  | [ |- appcontext[ (match ?X with Build_Eqv e _ _ _ => e end) ] ] => 
+      let X' := eval hnf in X in 
+      change X with X' ; 
+      cbv iota beta
+  end.
+
+Local Instance Eqv_WeakEqv {A} `{! Eqv A } : WeakEqv A :=
+  { weqv := eqv
+  ; WeakEqv_Symmetric := Eqv_Symmetric
+  ; WeakEqv_Transitive := Eqv_Transitive
+  }.
 
 Module Notation.
   Infix "≃" := eqv (no associativity, at level 70).
