src/FP/Classes/WeakEqv.v
@@ -1,4 +1,3 @@
-Require Import FP.Classes.Eqv.
 Require Import FP.Classes.Symmetric.
 Require Import FP.Classes.Transitive.
 Require Import FP.Data.Relation.
@@ -11,17 +10,27 @@ Class WeakEqv (A:Type) : Type :=
   ; WeakEqv_Transitive :> Transitive weqv
   }.
 Arguments weqv {A} {WeakEqv} _ _ : simpl never.
+Local Infix "≈" := weqv (no associativity, at level 70).
 
-Definition weqv_proper_l 
-  {A} `{! WeakEqv A } {x y:A} (p:weqv x y) 
-  : weqv x x := transitivity y p (symmetry p).
-Definition weqv_proper_r 
-  {A} `{! WeakEqv A } {x y:A} (p:weqv x y) 
-  : weqv y y := transitivity x (symmetry p) p.
+Ltac unfold_weqv :=
+  unfold weqv ;
+  match goal with
+  | [ |- appcontext[ (match ?X with Build_WeakEqv e _ _ => e end) ] ] => 
+      let X' := eval hnf in X in 
+      change X with X' ; 
+      cbv iota beta
+  end.
+
+Section proper.
+  Context {A} `{! WeakEqv A } {x y:A} (p:x ≈ y).
+  Definition weqv_proper_l : x ≈ x := transitivity y p (symmetry p).
+  Definition weqv_proper_r : y ≈ y := transitivity x (symmetry p) p.
+End proper.
+
 Ltac WeqvProper :=
   match goal with
-  | [ H : weqv ?x ?y |- weqv ?x ?x ] => apply (weqv_proper_l H)
-  | [ H : weqv ?x ?y |- weqv ?y ?y ] => apply (weqv_proper_r H)
+  | [ H : ?x ≈ ?y |- ?x ≈ ?x ] => apply (weqv_proper_l H)
+  | [ H : ?x ≈ ?y |- ?y ≈ ?y ] => apply (weqv_proper_r H)
   end.
 
 Instance Function_WeakEqv 
@@ -40,14 +49,21 @@ Defined.
 Section Function.
   Context {A B} `{! WeakEqv A ,! WeakEqv B}.
 
-  Definition function_weqv_app {f g:A -> B} (Rfg:weqv f g) {x y:A} (Rxy:weqv x y) 
-    : weqv (f x) (g y) := Rfg x y Rxy.
+  (* Respect introduction for _->_ *)
+  Definition fun_respect_intro
+    (f g:A -> B) (p:forall x y, x ≈ y -> f x ≈ g y)
+    : f ≈ g := p.
+
+  (* Respect elimination for _->_ *)
+  Definition fun_respect_elim
+    (f g:A -> B) (pf:f ≈ g) (x y:A) (px:x ≈ y)
+    : f x ≈ g y := pf x y px.
 End Function.
 
 Local Instance Leibniz_WeakEqv (T:Type) : WeakEqv T := { weqv := eq }.
 Proof.
-  constructor ; intros ; subst ; auto.
-  constructor ; intros ; subst ; auto.
+  - constructor ; intros ; subst ; auto.
+  - constructor ; intros ; subst ; auto.
 Defined.
     
 Module Notation.
