src/FP/Data/Function_Q.v
@@ -2,26 +2,16 @@ Require Import FP.Data.WeakSetoid.
 Require Import FP.Data.Function.
 Require Import FP.Data.Relation.
 Require Import FP.Classes.Eqv.
+Require Import FP.Data.Function.
+Require Import FP.Classes.WeakEqv.
 
 Import WeakSetoid.Notation.
 Import Eqv.Notation.
 Import WeakEqv.Notation.
+Import Function.Notation.
 
-Definition id_Q {A:WeakSetoid} : DD (A ⇨ A) := mk_DD_infer (A ⇨ A) id.
-
-Definition id_Q_beta {A:WeakSetoid} (x:DD A) : id_Q ⊛ x ≃ x.
-Proof. decide_weqv_beta. Qed.
-
-Definition compose_Q {A B C:WeakSetoid} : DD ((B ⇨ C) ⇨ (A ⇨ B) ⇨ (A ⇨ C)) :=
-  mk_DD_infer ((B ⇨ C) ⇨ (A ⇨ B) ⇨ A ⇨ C) compose.
-Definition compose_Q_beta {A B C:WeakSetoid} (g:DD (B ⇨ C)) (f:DD (A ⇨ B)) (x:DD A) 
-  : compose_Q ⊛ g ⊛ f ⊛ x ≃ g ⊛ (f ⊛ x).
-Proof. decide_weqv_beta. Defined.
-
-Definition apply_Q {A B:WeakSetoid} : DD ((A ⇨ B) ⇨ A ⇨ B) :=
-  mk_DD_infer ((A ⇨ B) ⇨ A ⇨ B) apply.
-
-Definition flip_Q {A B C:WeakSetoid} : DD ((A ⇨ B ⇨ C) ⇨ B ⇨ A ⇨ C) :=
-  mk_DD_infer ((A ⇨ B ⇨ C) ⇨ B ⇨ A ⇨ C) flip.
-
+Definition id_Q {A:WeakSetoid} : DD (A ⇨ A) := λ x → x.
+Definition compose_Q {A B C:WeakSetoid} : DD ((B ⇨ C) ⇨ (A ⇨ B) ⇨ (A ⇨ C)) := λ g f x → g ⊛ (f ⊛ x).
+Definition apply_Q {A B:WeakSetoid} : DD ((A ⇨ B) ⇨ A ⇨ B) := λ f x → f ⊛ x.
+Definition flip_Q {A B C:WeakSetoid} : DD ((A ⇨ B ⇨ C) ⇨ B ⇨ A ⇨ C) := λ f y x → f ⊛ x ⊛ y.
 Definition apply_to_Q {A B:WeakSetoid} : DD (A ⇨ (A ⇨ B) ⇨ B) := flip_Q ⊛ apply_Q.
