src/FP/Data/Tactic.v
@@ -1,2 +1,7 @@
 Tactic Notation "chain" tactic(t1) "|+|" tactic(t2) := ((t1 ; try t2) || t2).
 
+Ltac unfold_in_term name X :=
+  let X' := eval cbv beta delta[name] in X in
+  change X with X'.
+
+
